refactor(tc): use Turing.Tape.map for define forgetting
This allows to prove that stepping a ticking config is just like
stepping a normal config. This is a key feature to prove termination /
non-termination.

Busybeaver/Deciders/TranslatedCyclers.lean
@@ -11,24 +11,46 @@ abbrev TickingTape s := Turing.Tape (WithBot (Symbol s))
 instance TickingTape.inhabited: Inhabited (TickingTape s) :=
   ⟨{ head := (default : Symbol s), left := default, right := default }⟩
 
-abbrev LawfulTT s := { T: TickingTape s // T.head ≠ ⊥ }
-
-instance LawfulTT.inhabited: Inhabited (LawfulTT s) :=
-  ⟨default, by simp [default]⟩
-
 structure TickingConfig (l s) where
   state : Label l
-  tape : LawfulTT s
+  tape : TickingTape s
 
 instance TickingConfig.inhabited: Inhabited (TickingConfig l s) :=
   ⟨{state := default, tape := default}⟩
 
 abbrev Tick (l s) := Label l × (WithBot (Symbol s))
 
-def TickingTape.toLawful (T: TickingTape s): LawfulTT s := match h: T.head with
-| ⊥ => ⟨{T with head := (default: Symbol s)}, by simp⟩
-| some sym => ⟨T, by simp [h]⟩
+section ToBase
 
+/-
+To convert a ticking tape to a normal tape, with use Turing.Tape.map with a "forgetting" operation.
+
+We thus leverage the lemmas of Turing.Tape.move this way
+-/
+
+/- The "forgetting" pointed map -/
+def unbot_pointed [Inhabited α]: Turing.PointedMap (WithBot α) α := {
+  f := WithBot.unbot' default
+  map_pt' := rfl
+}
+
+def TickingTape.forget (T: TickingTape s): Turing.Tape (Symbol s) :=
+  T.map unbot_pointed
+
+def TickingConfig.toConfig (C: TickingConfig l s): Config l s := {
+  state := C.state,
+  tape := C.tape.forget
+}
+
+variable {C: TickingConfig l s}
+
+@[simp]
+lemma TickingConfig.toConfig.state: C.toConfig.state = C.state := rfl
+
+@[simp]
+lemma TickingConfig.toConfig.head: C.toConfig.tape.head = WithBot.unbot' default C.tape.head := rfl
+
+end ToBase
 
 section PrettyPrint
 open Std.Format Lean
@@ -42,20 +64,51 @@ private def left_repr [Repr α] [Inhabited α] (l: Turing.ListBlank α) (bound: 
 | n + 1 => left_repr l.tail n ++ [repr l.head]
 
 instance: Repr (TickingConfig l s) := ⟨λ cfg _ ↦
-  Std.Format.joinSep (left_repr cfg.tape.val.left 10) " " ++ s!" {cfg.state}>{repr cfg.tape.val.head} " ++ Std.Format.joinSep (right_repr cfg.tape.val.right 10) " "⟩
+  Std.Format.joinSep (left_repr cfg.tape.left 10) " " ++ s!" {cfg.state}>{repr cfg.tape.head} " ++ Std.Format.joinSep (right_repr cfg.tape.right 10) " "⟩
 
 end PrettyPrint
 
 
 def step_tick (M: Machine l s) (C: TickingConfig l s): Option (TickingConfig l s × Tick l s) :=
-  match hM: C.tape.val.head with
-  | none => by {
-    obtain ⟨Cs, Ct, CtH⟩ := C
-    simp at hM
-    contradiction
-  }
-  | some sym => match M C.state sym with
-    | .halt => .none
-    | .next sym' dir lab' =>
-      let t := (C.tape.val.write ↑sym').move dir
-      .some ({state := lab', tape := TickingTape.toLawful t }, (C.state, t.head))
+  let unboted: Symbol s := (WithBot.unbot' default C.tape.head)
+  match M C.state unboted with
+  | .halt => .none
+  | .next sym' dir lab' =>
+    .some ({state := lab', tape := (C.tape.write ↑sym').move dir }, (C.state, unboted))
+
+namespace TReach
+
+notation A " t-[" M ":" T "]-> " B => step_tick M A = Option.some (B, T)
+
+inductive MultiTStep (M: Machine l s): TickingConfig l s → TickingConfig l s → List (Tick l s) → Prop
+| refl C : MultiTStep M C C []
+| step A B C t L : (A t-[M:t]-> B) → MultiTStep M B C L → MultiTStep M A C (t :: L)
+
+notation A " t-[" M ":" L "]->> " B => MultiTStep M A B L
+
+lemma single_step {A B: TickingConfig l s} (h: A t-[M : t]-> B): A.toConfig -[M]-> B.toConfig :=
+by {
+  simp [step_tick] at h
+  split at h
+  · simp_all
+  rename_i heq
+  simp at h
+  obtain ⟨hB, _⟩ := h
+  simp [Machine.step]
+  split
+  · rename_i heq'
+    rw [heq] at heq'
+    cases heq'
+  rename_i heq'
+  rw [heq] at heq'
+  cases heq'
+  simp
+  rw [← hB]
+  simp [TickingConfig.toConfig, TickingTape.forget, Turing.Tape.map_move]
+  congr
+}
+
+lemma MultiTStep.to_multistep (h: A t-[M : L]->> B): A.toConfig -[M]{L.length}-> B.toConfig :=
+by induction h with
+| refl => exact .refl
+| step A B C t L hAB _ IH => exact Machine.Multistep.succ (single_step hAB) IH
